src/TCP.mli
@@ -1,0 +1,24 @@
+type socket
+
+val new_tcp_socket : string -> socket
+(** [new_tcp_socket addr] creates a [socket], where [addr] is of the
+    form {v [url]:[port] v}. *)
+
+val listen_incoming_connection : socket -> unit
+(** [listen_incoming_connection sck] changes the mode of the socket
+    [sck], effectively creating a server. *)
+
+val accept_connection : socket -> socket
+(** [accept_connection sck] waits for [sck] to receive an incoming connection,
+    and returns a [socket] to interact with the new client. *)
+
+val read_socket : socket -> string
+(** [read_socket sck] waits for the client behind [sck] to send data
+    (interpreted as a [string]). *)
+
+val write_socket : socket -> string -> unit
+(** [write_socket sck msg] sends [msg] to the client behind [sck]. *)
+
+val close_tcp_socket : socket -> unit
+(** [close_tcp_socket sck] interupts an existing connection by closing
+    the link between the server and the client. *)
