src/console.ml
@@ -1,0 +1,3 @@
+let echo = print_string
+
+let scan = read_line
