src/console.mli
@@ -1,0 +1,3 @@
+val echo : string -> unit
+
+val scan : unit -> string
