src/fileSystem.ml
@@ -18,53 +18,12 @@
  * along with this program. If not, see <http://www.gnu.org/licenses/>.
  *)
 
-open Freespec_exec.Coqstr
-open Freespec_exec.Coqbool
-open Freespec_exec.Extends
-open Freespec_exec.Coqunit
-open ExtUnix
+type file = Unix.file_descr
 
-let path = "minihttpserver.filesystem"
+let open_file path = Unix.openfile path [ O_RDONLY ] 0
 
-let constr_of_fd fd =
-  Constr.(of_kind (Int (Uint63.of_int (Obj.magic fd))))
+let file_exists = Sys.file_exists
 
-let fd_of_constr c =
-  match Constr.kind c with
-  | Constr.Int i -> (Obj.magic (snd (Uint63.to_int2 i)) : Unix.file_descr)
-  | _ -> assert false
+let read_file = ExtUnix.read_all_from ~line:false
 
-let open_file = function
-  | [path] ->
-     Unix.openfile (string_of_coqbytes path) [ O_RDONLY ] 0 |> constr_of_fd
-  | _ ->
-     assert false
-
-let file_exists = function
-  | [path] ->
-     Sys.file_exists (string_of_coqbytes path)
-     |> bool_to_coqbool
-  | _ ->
-     assert false
-
-let read_file = function
-  | [fd] ->
-     read_all_from ~line:false (fd_of_constr fd) |>
-     string_to_coqbytes
-  | _ ->
-     assert false
-
-let close_file = function
-  | [fd] ->
-     Unix.close (fd_of_constr fd);
-     coqtt
-  | _ ->
-     assert false
-
-let install_interface =
-  register_interface path [
-      ("Open",   open_file);
-      ("FileExists", file_exists);
-      ("Read",   read_file);
-      ("Close",  close_file)
-    ]
+let close_file = Unix.close 
