src/fileSystem.mli
@@ -1,0 +1,6 @@
+type file
+
+val open_file : string -> file
+val file_exists : string -> bool
+val read_file : file -> string
+val close_file : file -> unit
