src/slice.ml
@@ -1,0 +1,30 @@
+type t = { str_buffer : string; str_offset : int; str_len : int }
+
+let of_string s = { str_buffer = s; str_offset = 0; str_len = String.length s }
+
+let to_string { str_buffer; str_offset; str_len } =
+  if str_len = String.length str_buffer then str_buffer
+  else String.init str_len (fun idx -> String.get str_buffer (idx + str_offset))
+
+let of_char c = Strext.char_to_string c |> of_string
+
+let length t = t.str_len
+
+let unpack { str_buffer; str_offset; str_len } =
+  if 0 < str_len then
+    Some
+      ( String.get str_buffer str_offset,
+        { str_buffer; str_offset = str_offset + 1; str_len = str_len - 1 } )
+  else None
+
+let take { str_buffer; str_offset; str_len } x =
+  if x <= str_len then
+    Some
+      ( { str_buffer; str_offset; str_len = x },
+        { str_buffer; str_offset = str_offset + x; str_len = str_len - x } )
+  else None
+
+let pack l =
+  let str_len = List.length l in
+  let str_buffer = String.init str_len (List.nth l) in
+  { str_buffer; str_offset = 0; str_len }
