src/slice.mli
@@ -1,0 +1,15 @@
+type t
+
+val of_string : string -> t
+
+val of_char : char -> t
+
+val to_string : t -> string
+
+val length : t -> int
+
+val unpack : t -> (char * t) option
+
+val take : t -> int -> (t * t) option
+
+val pack : char list -> t
