src/strext.ml
@@ -1,0 +1,5 @@
+let of_int i = Format.sprintf "%d" i
+
+let char_to_string x = String.make 1 x
+
+let length = String.length
