src/strext.mli
@@ -1,0 +1,5 @@
+val of_int : int -> string
+
+val char_to_string : char -> string
+
+val length : string -> int
