theories/HTTP.v
@@ -1,6 +1,9 @@
-From Prelude Require Import All Bytes Byte Int.
 From Comparse Require Import Monad Combinators.
+From MiniHTTPServerFFI Require Import Slice SliceFacts StrExt.
 From MiniHTTPServer Require Import URI.
+From CoqFFI Require Import String.
+
+Import MonadLetNotation.
 
 Inductive request :=
 | Get (resource : uri).
@@ -10,7 +13,7 @@ Inductive status :=
 | client_error_BadRequest
 | client_error_NotFound.
 
-Definition status_to_bytes (code : status) : bytes :=
+Definition status_to_bytes (code : status) : string :=
   match code with
   | success_OK => "200"
   | client_error_BadRequest => "400"
@@ -18,18 +21,23 @@ Definition status_to_bytes (code : status) : bytes :=
   end.
 
 Record response := make_response { code : status
-                                 ; body : bytes
+                                 ; body : string
                                  }.
 
-Definition whitespaces : parser bytes unit :=
-  skip (many (char c#" ")).
+Definition whitespaces : parser Slice.t unit :=
+  skip (many (char " ")).
 
-Definition http_request : parser bytes request :=
-  Get <$> (str "GET" *> whitespaces *> read_uri <* whitespaces <* str "HTTP/1.1").
+Definition http_request : parser Slice.t request :=
+  str "GET";;
+  whitespaces;;
+  let* uri := read_uri in
+  whitespaces;;
+  str "HTTP/1.1";;
+  pure (Get uri).
 
-Definition response_to_string (res : response) : bytes :=
+Definition response_to_string (res : response) : string :=
   "HTTP/1.1 " ++ status_to_bytes (code res) ++ " Response\r\n" ++
-  "Content-Length: " ++ (bytes_of_int (Bytes.length (body res))) ++ "\r\n" ++
+  "Content-Length: " ++ (StrExt.of_int (StrExt.length (body res))) ++ "\r\n" ++
   "Connection: Closed\r\n" ++
   "\r\n" ++
   body res ++ "\r\n" ++
