main.v
@@ -1,4 +1,0 @@
-From FreeSpec Require Import Exec.
-From MiniHTTPServer Require Import App Exec.
-
-Exec (http_server 100).
