src/SliceFacts.v
@@ -1,0 +1,14 @@
+From MiniHTTPServerFFI Require Import Slice StrExt.
+From Comparse Require Import Monad Combinators.
+
+Instance slice_input : Input Slice.t ascii :=
+  { unpack := Slice.unpack
+  ; input_to_string := Slice.to_string
+  ; token_to_string := StrExt.char_to_string
+  }.
+
+Axiom slice_length : Slice.t -> nat.
+
+Axiom slice_laws : InputLaws Slice.t ascii slice_length.
+
+#[global] Existing Instance slice_laws.
